ITree_Circus.thy
@@ -14,7 +14,7 @@ definition Skip :: "('e, 'r) htree" where
 
 expr_ctr subst_id
 
-lemma straces_Skip: "traces\<^sub>s (Skip) = ({[], [\<cmark> [\<leadsto>]]})\<^sub>e"
+lemma straces_Skip: "traces\<^sub>s (Skip) = ({[], [\<checkmark> [\<leadsto>]]})\<^sub>e"
   by (simp add: Skip_def straces_def traces_Ret, expr_simp)
 
 abbreviation Div :: "('e, 'r) htree" where
@@ -75,7 +75,7 @@ translations
   "_assignment x e" == "CONST assigns (CONST subst_upd (CONST subst_id) x (e)\<^sub>e)"
   "_assignment (_svid_tuple (_of_svid_list (x +\<^sub>L y))) e" <= "_assignment (x +\<^sub>L y) e"
 
-lemma traces_inp: "wb_prism c \<Longrightarrow> traces (inp c) = {[]} \<union> {[Ev (build\<^bsub>c\<^esub> v)] | v. True} \<union> {[Ev (build\<^bsub>c\<^esub> v), \<cmark> v] | v. True}" 
+lemma traces_inp: "wb_prism c \<Longrightarrow> traces (inp c) = {[]} \<union> {[Ev (build\<^bsub>c\<^esub> v)] | v. True} \<union> {[Ev (build\<^bsub>c\<^esub> v), \<checkmark> v] | v. True}" 
   apply (simp add: inp_in_where_def traces_Vis traces_Ret)
   apply (auto simp add: inp_in_where_def bind_eq_Some_conv traces_Ret domIff pdom.abs_eq  elim!: in_tracesE trace_to_VisE)
   done 
