examples/DwarfSignal.thy
@@ -125,47 +125,6 @@ definition "DwarfSignal
 
 simulate DwarfSignal
 
-
-ML \<open> Code.read_const @{theory} "DwarfSignal" \<close>
-
-ML \<open> 
-
-
-\<close>
-
-local_setup \<open>
-  ITree_Simulator.simulate "DwarfSignal"
-\<close>
-
-local_setup \<open> 
-Code_Target.export_code true [@{const_name DwarfSignal}] [((("Haskell", ""), SOME ({physical = false}, (Path.explode "simulate", Position.none))), (Token.explode (Thy_Header.get_keywords' @{context}) Position.none "string_classes"))] 
-#>
-ITree_Simulator.prep_simulation "DwarfSignal"
-\<close>
-
-(* [(("Haskell", ""), SOME ({physical = false}, (Path.explode "simulate", Position.none)), [])] *)
-
-(*
-local_setup \<open>
-fn ctx =>
-  Generated_Files.generate_file (Path.binding0 (Path.make ["code", "simulate", "Simulation.hs"]), \<open>\<close>) ctx |>
-  (fn ctx => let val _ = Generated_Files.export_generated_files ctx [([], Local_Theory.exit_global ctx)] in ctx end)
-\<close>
-*)
-
-local_setup \<open>  \<close>
-
-
-                          
-ML \<open> ITree_Simulator.run_simulation @{theory} \<close>
-(*
-compile_generated_files _ and "code/simulate/Simulate.hs" (in ITree_Simulation) where 
-\<open>     fn path => let val n = @{print} (Path.implode path); val ret = Isabelle_System.bash ("/home/simonfoster/Isabelle/simulate.sh " ^ n ^ "/code/simulate"  ^ " DwarfSignal.hs") in  () end
-  \<close>
-*)
-
-ML \<open> Isabelle_System.getenv "ISABELLE_TMP" \<close>
-
 text \<open> Testing SML lazy code evaluation \<close>
 
 code_lazy_type itree
